nr: states for the advance tail transitions
Signed-off-by: Reto Achermann <achreto@gmail.com>

concurrency/node-replication/CyclicBuffer.i.dfy
@@ -4,34 +4,293 @@ include "../framework/Cells.s.dfy"
 include "../framework/GlinearOption.s.dfy"
 include "Constants.i.dfy"
 
-module CyclicBufferRw(nrifc:  refines MultiRw {
+
+module CyclicBufferRw(nrifc: NRIfc) refines MultiRw {
   type Key(!new) = nat
+
   glinear datatype StoredType = StoredType(
     glinear cellContents: CellContents<LogEntry>,
     glinear logEntry: glOption<Log>
   )
 
-  datatype AdvanceHeadState = AdvanceHeadState(idx: nat, min_tail: nat)
+  datatype AdvanceHeadState =
+    | AdvanceHeadIdle
+    | AdvHeadNextLoaded(next: NodeId)
+    | AdvHeadHeadLoaded(next: NodeId, head : nat)
+    | AdvHeadMinLtail(next: NodeId, head: nat, mintail: nat, idx: NodeId)
+
   datatype AdvanceTailState = AdvanceTailState(obvserve_head: nat)
   datatype AppendState = AppendState(cur_idx: nat, tail: nat)
 
+  // define the nodeid type
+  type NodeId = nat
+
+  // Corresponds to: pub struct Log<'a, T>
   datatype M =
     | MInvalid
     | M(
+      // Logical index into the above slice at which the log starts.
       head: Option<nat>,
-      globalTail: Option<nat>,
-      localTails: map<nat, nat>,
+      // Logical index into the above slice at which the log ends.
+      // New appends go here.
+      tail: Option<nat>,
+
+      // Completed tail maintains an index <= tail that points to a
+      // log entry after which there are no completed operations across
+      // all replicas registered against this log.
+      // TODO(RA): do we need this?
+      // ctail: Option<nat>,
+
+      // Array consisting of the local tail of each replica registered with the log.
+      // Required for garbage collection; since replicas make progress over the log
+      // independently, we want to make sure that we don't garbage collect operations
+      // that haven't been executed by all replicas.
+      ltails: map<NodeId, nat>,
+
+      // Identifier that will be allocated to the next replica that registers with
+      // this Log. Also required to correctly index into ltails above.
+      next: Option<NodeId>,
+
+      /// Array consisting of local alive masks for each registered replica. Required
+      /// because replicas make independent progress over the log, so we need to
+      /// track log wrap-arounds for each of them separately.
+      lmasks: map<NodeId, bool>,
+
+      /// The maximum number of entries that can be held inside the log.
+      size: Option<nat>,
+
+      /// A reference to the actual log. Nothing but a slice of entries.
+      // slog: &'a [Cell<Entry<T>>],
       contents: map<int, StoredType>,
+
+
       // TODO: could we have multiple threads advancing the head, we assume so
-      advanceHead: map<nat, AdvanceHeadState>,
-      advanceTail: map<nat, AdvanceTailState>,
-      appendState: map<nat, AppendState>,
+      advanceHead: map<NodeId, AdvanceHeadState>,
+      advanceTail: map<NodeId, AdvanceTailState>,
+      appendState: map<NodeId, AppendState>
     )
 
   function dot(x: M, y: M) : M
   function unit() : M
 
   predicate Init(s: M)
-  predicate Inv(x: M) 
+  predicate Inv(x: M)
   function I(x: M) : map<Key, StoredType> requires Inv(x)
+
+  /////////////////////////////////////////////////////////////////////////////
+  // State Guards
+  /////////////////////////////////////////////////////////////////////////////
+
+  predicate StateValid(m: M) {
+    m.M?
+  }
+
+  predicate NextFieldValid(m: M)
+    requires StateValid(m)
+  {
+    m.next.Some?
+  }
+
+  predicate HeadFieldValid(m: M)
+    requires StateValid(m)
+  {
+    m.head.Some?
+  }
+
+  predicate TailFieldValid(m: M)
+    requires StateValid(m)
+  {
+    m.tail.Some?
+  }
+
+  /////////////////////////////////////////////////////////////////////////////
+  // Advance Head Guards
+  /////////////////////////////////////////////////////////////////////////////
+
+  // we're in the advance head idle state
+  predicate AdvHeadInIdle(m: M, nodeId: NodeId)
+    requires StateValid(m)
+  {
+    && nodeId in m.advanceHead
+    && m.advanceHead[nodeId].AdvanceHeadIdle?
+  }
+
+  predicate AdvHeadInNextLoaded(m: M, nodeId: NodeId)
+    requires StateValid(m)
+  {
+    && nodeId in m.advanceHead
+    && m.advanceHead[nodeId].AdvHeadNextLoaded?
+  }
+
+  predicate AdvHeadInReadHead(m: M, nodeId: NodeId)
+    requires StateValid(m)
+  {
+    && nodeId in m.advanceHead
+    && m.advanceHead[nodeId].AdvHeadHeadLoaded?
+  }
+
+  predicate AdvHeadInMinLTail(m: M, nodeId: NodeId)
+    requires StateValid(m)
+  {
+    && nodeId in m.advanceHead
+    && m.advanceHead[nodeId].AdvHeadMinLtail?
+    && m.advanceHead[nodeId].idx < m.advanceHead[nodeId].next
+  }
+
+  predicate AdvHeadMinLtailValid(m: M, nodeId: NodeId)
+    requires AdvHeadInMinLTail(m, nodeId)
+  {
+    && var st := m.advanceHead[nodeId];
+    && st.idx in m.LocalTails
+  }
+
+  predicate AdvHeadInMinLTailDone(m: M, nodeId: NodeId)
+    requires StateValid(m)
+  {
+    && nodeId in m.advanceHead
+    && m.advanceHead[nodeId].AdvHeadMinLtail?
+    && m.advanceHead[nodeId].idx == m.advanceHead[nodeId].next
+  }
+
+
+
+  /////////////////////////////////////////////////////////////////////////////
+  // Reading Transitions
+  /////////////////////////////////////////////////////////////////////////////
+
+  //
+  //
+  //
+  //
+
+
+  /////////////////////////////////////////////////////////////////////////////
+  // Append Transitions
+  /////////////////////////////////////////////////////////////////////////////
+
+  // pub fn append<F: FnMut(T, usize)>(&self, ops: &[T], idx: usize, mut s: F)
+
+  /////////////////////////////////////////////////////////////////////////////
+  // AdvanceHead Transitions
+  /////////////////////////////////////////////////////////////////////////////
+
+  // fn advance_head<F: FnMut(T, usize)>(&self, rid: usize, mut s: &mut F);
+
+  // { AdvHeadIdle }
+  //   let r = self.next.load(Ordering::Relaxed);
+  // { AdvHeadNextLoaded(next) }
+  predicate TransitionAdvHeadLoadNext(m: M, m': M, nodeId: NodeId) {
+    && StateValid(m)
+    && AdvHeadInIdle(m, nodeId)
+    && NextFieldValid(m)
+
+    // read the next field
+    && var next := m.next.value;
+
+    // construct the new state
+    && var newst := AdvHeadNextLoaded(next);
+
+    // update the state of the advanceHead
+    && m' == m.(advanceHead := m.advanceHead[ nodeId :=  newst])
+  }
+
+  // { AdvHeadNextLoaded(next) }
+  //   let global_head = self.head.load(Ordering::Relaxed);
+  // { AdvHeadHeadLoaded(next, head) }
+  predicate TransitionAdvHeadReadHead(m: M, m': M, nodeId: NodeId) {
+    && StateValid(m)
+    && AdvHeadInNextLoaded(m, nodeId)
+    && HeadFieldValid(m)
+
+    // get the old state
+    && var st := m.advanceHead[nodeId];
+
+    // read the next field
+    && var head := m.head.value;
+
+    // construct the new state
+    && var newst := AdvHeadNextLoaded(st.next, head);
+
+    // update the state of the advanceHead
+    && m' == m.(advanceHead := m.advanceHead[ nodeId :=  newst])
+  }
+
+
+  // let f = self.tail.load(Ordering::Relaxed);
+  // that one seems to be no-where used??
+
+  // { AdvHeadHeadLoaded(next, head) }
+  //   let mut min_local_tail = self.ltails[0].load(Ordering::Relaxed);
+  // { AdvHeadMinLtail(next, head, min_local_tail, idx = 1) }
+  predicate TransitionAdvHeadMinLTail(m: M, m': M, nodeId: NodeId) {
+    && StateValid(m)
+    && AdvHeadInReadHead(m, nodeId)
+    && 0 in m.localTails
+
+    // get the old state
+    && var st := m.advanceHead[nodeId];
+
+    // read the first local tail
+    && var ltail := m.localTails[0];
+
+    // construct the new state
+    && var newst := AdvHeadMinLtail(st.next, st.head, ltail, 1);
+
+    // update the state of the advanceHead
+    && m' == m.(advanceHead := m.advanceHead[ nodeId :=  newst])
+  }
+
+
+  // { AdvHeadMinLtail(next, head, min_local_tail, idx = 1)
+  //   for idx in 1..r {
+  //     let cur_local_tail = self.ltails[idx - 1].load(Ordering::Relaxed);
+  //     if min_local_tail > cur_local_tail {
+  //         min_local_tail = cur_local_tail
+  //     };
+  //   }
+  // assert(idx == next)
+  // { AdvHeadMinLtail(next, head, min_local_tail, idx = next)
+  predicate TransitionAdvHeadMinLTailNext(m: M, m': M, nodeId: NodeId) {
+    && StateValid(m)
+    && AdvHeadInMinLTail(m, nodeId)
+    && AdvHeadMinLtailValid(m, nodeId)
+
+    // get the old state
+    && var st := m.advanceHead[nodeId];
+
+    // read the current local tail
+    && var cur_local_tail := m.localTails[st.idx];
+
+    // if the current local tail is smaller, update the value
+    && var ltail := if st.mintail > cur_local_tail then cur_local_tail else st.mintail;
+
+    // construct the new state
+    && var newst := AdvHeadMinLtail(st.next, st.head, ltail, st.idx + 1);
+
+    // update the state of the advanceHead
+    && m' == m.(advanceHead := m.advanceHead[ nodeId :=  newst])
+  }
+
+  // What About the exec stuff here?
+  // { AdvHeadMinLtail(next, head, min_local_tail, idx = next)
+  //   self.head.store(min_local_tail, Ordering::Relaxed);
+  // { AdvHeadIdle }
+  predicate TransitionAdvHeadIdle(m: M, m': M, nodeId: NodeId) {
+    && StateValid(m)
+    && AdvHeadInMinLTailDone(m, nodeId)
+
+    // get the old state
+    && var st := m.advanceHead[nodeId];
+
+    // the new head value
+    && var new_head := st.mintail;
+
+    // construct the new state
+    && var newst := AdvHeadIdle;
+
+    // update the state of the advanceHead
+    && m' == m.(advanceHead := m.advanceHead[ nodeId :=  newst])
+              .(head := Some(new_head))
+  }
+
 }
